examples/pseudo_bool/array/README.md
@@ -1,0 +1,22 @@
+Improving the pseudoboolean proof checker with arrays (manually)
+
+[cnfProgScript.sml](cnfProgScript.sml):
+CNF encoder and checker
+
+[compilation](compilation):
+Compiling the pseudo-boolean constraints checker
+
+[npbc_arrayProgScript.sml](npbc_arrayProgScript.sml):
+Refine npbc_list to npbc_array
+
+[npbc_fullProgScript.sml](npbc_fullProgScript.sml):
+Add PBF parsing and wrap around the PBP parser
+
+[npbc_listScript.sml](npbc_listScript.sml):
+Refine PB proof checker to use arrays
+
+[npbc_parseProgScript.sml](npbc_parseProgScript.sml):
+Add shared pbp parsing, normalization and other common stuff to npbc_arrayProg
+
+[subgraph_isoProgScript.sml](subgraph_isoProgScript.sml):
+Subgraph isomorphism encoder and checker
