examples/pseudo_bool/array/compilation/README.md
@@ -1,0 +1,10 @@
+Compiling the pseudo-boolean constraints checker
+
+[cnfCompileScript.sml](cnfCompileScript.sml):
+Compiles the encoder
+
+[npbc_fullCompileScript.sml](npbc_fullCompileScript.sml):
+Compiles the PB checker example by evaluation inside the logic of HOL
+
+[subgraph_isoCompileScript.sml](subgraph_isoCompileScript.sml):
+Compiles the encoder
